intermediate/Veritas.Intermediate.StoreSKC.fst
@@ -13,72 +13,143 @@ let store_contains_st_index (st:vstore) (s:slot_id{store_contains st s})
   = ()
 
 let stored_key (st:vstore) (s:slot_id{store_contains st s}) : key
-  = VStore?.k (Some?.v (get_slot st s))
+  = VStoreE?.k (Some?.v (get_slot st s))
 
 let stored_value (st:vstore) (s:slot_id{store_contains st s}) : value
-  = VStore?.v (Some?.v (get_slot st s))
+  = VStoreE?.v (Some?.v (get_slot st s))
 
 let stored_value_matches_stored_key (st:vstore) (s:slot_id{store_contains st s}) 
   : Lemma (is_value_of (stored_key st s) (stored_value st s))
   = ()
 
 let add_method_of (st:vstore) (s:slot_id{store_contains st s}) : add_method
-  = VStore?.am (Some?.v (get_slot st s))
+  = VStoreE?.am (Some?.v (get_slot st s))
 
 let lookup_key (st:vstore) (k:key) 
   : option vstore_entry
   = let f ro = if None? ro then false
-               else let Some r = ro in VStore?.k r = k in
-    let s = filter f st.data in
-    if Seq.length s = 0 then None
-    else Seq.index s 0 
+               else let Some r = ro in r.k = k in
+    let s' = filter f st.data in
+    if Seq.length s' = 0 then None
+    else Seq.index s' 0 
 
 let store_contains_key (st:vstore) (k:key) : bool
   = Some? (lookup_key st k)
 
-let lemma_lookup_key (st:vstore) (k:key) 
+let lemma_lookup_key_returns_k (st:vstore) (k:key) 
   : Lemma (requires (store_contains_key st k))
-          (ensures (VStore?.k (Some?.v (lookup_key st k)) = k))
+          (ensures (VStoreE?.k (Some?.v (lookup_key st k)) = k))
   = let f ro = if None? ro then false
-               else let Some r = ro in VStore?.k r = k in
+               else let Some r = ro in r.k = k in
     lemma_filter_correct1 f st.data 0
+
+let lemma_lookup_key_returns_None (st:vstore) (k:key)
+  : Lemma (requires (lookup_key st k = None))
+          (ensures (let f ro = if None? ro then false
+                               else let Some r = ro in r.k = k in
+                    forall i. not (f (Seq.index st.data i))))
+  = let f ro = if None? ro then false
+               else let Some r = ro in r.k = k in
+    let s' = filter f st.data in
+    if Seq.length s' = 0 
+    then lemma_filter_all_not f st.data
+    else lemma_filter_correct1 f st.data 0
 
 let lemma_store_contains_key (st:vstore) (k:key)
   : Lemma (requires (exists s. stored_key st s = k))
           (ensures (store_contains_key st k))
   = let f ro = if None? ro then false
-               else let Some r = ro in VStore?.k r = k in
+               else let Some r = ro in r.k = k in
     lemma_filter_exists f st.data;
     lemma_filter_correct1 f st.data 0
 
+(* Opposite direction of previous lemma *)
+let lemma_store_contains_key_inv (st:vstore) (k:key)
+  : Lemma (requires (store_contains_key st k))
+          (ensures (exists s. stored_key st s = k))
+  = let f ro = if None? ro then false
+               else let Some r = ro in r.k = k in
+    let s' = filter f st.data in
+    if Seq.length s' > 0 
+    then 
+      let i = filter_index_map f st.data 0 in
+      assert (stored_key st i = k)
+
+let lemma_get_slot_lookup_key (st:vstore{st.is_map}) (s:slot_id) (k:key)
+  : Lemma (requires (store_contains st s /\ stored_key st s = k))
+          (ensures (get_slot st s = lookup_key st k))
+  = // relies on the fact that (filter f st.data) returns a unique elmt
+    admit()
+
 let stored_value_by_key (st:vstore) (k:key{store_contains_key st k})
   : value_type_of k
-  = lemma_lookup_key st k;
-    VStore?.v (Some?.v (lookup_key st k))
+  = lemma_lookup_key_returns_k st k;
+    VStoreE?.v (Some?.v (lookup_key st k))
 
 let add_method_of_by_key (st:vstore) (k:key{store_contains_key st k})
   : add_method
-  = VStore?.am (Some?.v (lookup_key st k))
+  = VStoreE?.am (Some?.v (lookup_key st k))
 
-let update_slot (st:vstore) (s:st_index st) (e:vstore_entry)
+(* Two cases where it's safe to add an entry (e) to the store (st) at s: 
+   * e.k is not in st
+   * e.k is already at s *)
+let compatible_entry (st:vstore) (s:st_index st) (e:vstore_entry) : Type
+  = not (store_contains_key st e.k) \/ 
+    (store_contains st s /\ stored_key st s = e.k) 
+
+let lemma_not_contains_key (st:vstore) (k:key) (s:slot_id{store_contains st s})
+  : Lemma (requires (not (store_contains_key st k)))
+          (ensures (stored_key st s <> k))
+  = ()
+
+let lemma_add_entry_case_1 (st:vstore) (s:st_index st) (e:vstore_entry)
+  : Lemma (requires (st.is_map /\ not (store_contains_key st e.k)))
+          (ensures (is_map_f (Seq.upd st.data s (Some e))))
+  = let l = Seq.upd st.data s (Some e) in
+    let aux (i:seq_index l{Some? (Seq.index l i)})
+            (i':seq_index l{Some? (Seq.index l i') /\ i <> i'})
+          : Lemma (VStoreE?.k (Some?.v (Seq.index l i)) <> VStoreE?.k (Some?.v (Seq.index l i')))
+                  [SMTPat (Seq.index l i); SMTPat (Seq.index l i')]
+          = if i = s 
+            then lemma_not_contains_key st e.k i' 
+            else if i' = s 
+                 then lemma_not_contains_key st e.k i in
+    assert (is_map_f l)
+
+let lemma_add_entry_case_2 (st:vstore) (s:st_index st) (e:vstore_entry)
+  : Lemma (requires (st.is_map /\ store_contains st s /\ stored_key st s = e.k))
+          (ensures (is_map_f (Seq.upd st.data s (Some e))))
+  = () 
+
+let update_slot (st:vstore) (s:st_index st) (e:vstore_entry{compatible_entry st s e})
   : vstore
-  = { st with data = Seq.upd st.data s (Some e) }
+  = if st.is_map 
+    then if not (store_contains_key st e.k) 
+         then lemma_add_entry_case_1 st s e 
+         else if store_contains st s && stored_key st s = e.k
+              then lemma_add_entry_case_2 st s e;
+    VStore (Seq.upd st.data s (Some e)) st.is_map
 
 let update_store 
-  (st:vstore) 
+  (st:vstore)
   (s:slot_id{store_contains st s}) 
   (v:value_type_of (stored_key st s))
   : Tot (st':vstore {store_contains st' s /\
                      stored_value st' s = v})
-  = let Some (VStore k _ am) = get_slot st s in
-    update_slot st s (VStore k v am) 
-
+  = let Some (VStoreE k _ am) = get_slot st s in
+    update_slot st s (VStoreE k v am) 
+  
 let update_store_preserves_length 
       (st:vstore) 
       (s:slot_id{store_contains st s}) 
       (v:value_type_of (stored_key st s)) 
   : Lemma (let st' = update_store st s v in
            Seq.length st.data = Seq.length st'.data)
+  = ()
+
+let lemma_update_store_preserves_is_map (st:vstore) s v
+  : Lemma (let st' = update_store st s v in 
+           st.is_map = st'.is_map)
   = ()
 
 let add_to_store 
@@ -91,13 +162,28 @@ let add_to_store
                      stored_key st' s = k /\
                      stored_value st' s = v /\
                      add_method_of st' s = am})
-  = update_slot st s (VStore k v am)
+  = let e = VStoreE k v am in
+    if not (store_contains_key st k)
+    then update_slot st s e
+    else VStore (Seq.upd st.data s (Some e)) false
+
+let lemma_add_to_store_is_map1 (st:vstore) s k v am
+  : Lemma (requires (not (store_contains_key st k)))
+          (ensures (let st' = add_to_store st s k v am in 
+                    st.is_map = st'.is_map))
+  = ()
+
+let lemma_add_to_store_is_map2 (st:vstore) s k v am
+  : Lemma (requires (store_contains_key st k))
+          (ensures (let st' = add_to_store st s k v am in 
+                    st'.is_map = false))
+  = ()
 
 let evict_from_store (st:vstore) (s:st_index st)
   : Tot (st':vstore {not (store_contains st' s)})
-  = { st with data = Seq.upd st.data s None }
+  = VStore (Seq.upd st.data s None) st.is_map
 
-let rec as_map_aux (l:Seq.seq (option vstore_entry)) 
+let rec as_map_aux (l:vstore_data) 
   : Tot Spec.vstore (decreases (Seq.length l)) =
   let n = Seq.length l in
   if n = 0 then fun _ -> None
@@ -106,19 +192,37 @@ let rec as_map_aux (l:Seq.seq (option vstore_entry))
     let f' = as_map_aux l' in
     match Seq.index l (n - 1) with
     | None -> f'
-    | Some (VStore k v a) -> 
+    | Some (VStoreE k v a) -> 
       fun (k':key) -> if k = k' then Some (Spec.VStore v a) else f' k' 
 
 let as_map (st:vstore{st.is_map}) : Spec.vstore =
   as_map_aux st.data
 
+let rec lemma_as_map_empty (n:nat) 
+  : Lemma (ensures (let st = VStore (Seq.create n None) true in
+                     forall (k:key). as_map st k = None))
+          (decreases n)
+  = if n <> 0 
+    then (
+      lemma_prefix_create n (None #vstore_entry) (n-1);
+      lemma_as_map_empty (n-1)
+    )
+
+let lemma_is_map_f_prefix (l:vstore_data) (i:seq_index l)
+  : Lemma (requires (is_map_f l))
+          (ensures (is_map_f (prefix l i)))
+          [SMTPat (is_map_f (prefix l i))]
+  = ()
+
 let rec lemma_as_map_slot_key_equiv_aux 
-      (l:Seq.seq (option vstore_entry)) 
-      (s:seq_index l) 
+      (l:vstore_data) 
+      (s:slot_id) 
       (k:key) 
       (v:value_type_of k) 
       (am:add_method)
-  : Lemma (requires (Seq.index l s = Some (VStore k v am))) 
+  : Lemma (requires (s < Seq.length l /\ 
+                     Seq.index l s = Some (VStoreE k v am) /\
+                     is_map_f l)) 
           (ensures (Spec.store_contains (as_map_aux l) k /\
                     Spec.stored_value (as_map_aux l) k = v))
           (decreases (Seq.length l))
@@ -126,20 +230,62 @@ let rec lemma_as_map_slot_key_equiv_aux
     if n <> 0 
     then
       let l' = prefix l (n - 1) in
-      let f' = as_map_aux l' in
       match Seq.index l (n - 1) with
       | None -> lemma_as_map_slot_key_equiv_aux l' s k v am
-      | Some (VStore _ _ _) -> 
+      | Some (VStoreE k2 v2 am2) -> 
           if s < n - 1 
-          then (
-                 lemma_as_map_slot_key_equiv_aux l' s k v am;
-                 // I thought the recursive call would work...
-                 admit()
-               )
+          then lemma_as_map_slot_key_equiv_aux l' s k v am
 
 let lemma_as_map_slot_key_equiv (st:vstore{st.is_map}) (s:slot_id) (k:key)
   : Lemma (requires (slot_key_equiv st s k)) 
           (ensures (Spec.store_contains (as_map st) k /\
                     stored_value st s = Spec.stored_value (as_map st) k)) 
-  = let Some (VStore k v a) = get_slot st s in 
+  = let Some (VStoreE k v a) = get_slot st s in 
     lemma_as_map_slot_key_equiv_aux st.data s k v a
+
+let rec lemma_as_map_aux_does_not_contain_key 
+      (l:vstore_data) 
+      (k:key) 
+  : Lemma (requires (let f ro = if None? ro then false
+                                else let Some r = ro in r.k = k in
+                     forall i. not (f (Seq.index l i)))) 
+          (ensures (not (Spec.store_contains (as_map_aux l) k)))
+          (decreases (Seq.length l))
+  = let n = Seq.length l in
+    if n <> 0 
+    then
+      let l' = prefix l (n - 1) in
+      lemma_as_map_aux_does_not_contain_key l' k
+
+let lemma_as_map_contains_key (st:vstore{st.is_map}) (k:key)
+  : Lemma (store_contains_key st k = Spec.store_contains (as_map st) k)
+  = if store_contains_key st k
+    then (
+      lemma_store_contains_key_inv st k;
+      Classical.exists_elim 
+        (Spec.store_contains (as_map st) k) 
+        (Squash.get_proof (exists s. slot_key_equiv st s k)) 
+        (fun s -> lemma_as_map_slot_key_equiv st s k)
+    )
+    else (
+      let f ro = if None? ro then false
+                 else let Some r = ro in r.k = k in
+      lemma_lookup_key_returns_None st k;
+      lemma_as_map_aux_does_not_contain_key st.data k
+    )
+
+let lemma_slot_key_equiv_value (st:vstore{st.is_map}) (s:slot_id) (k:key)
+  : Lemma (requires (slot_key_equiv st s k))
+          (ensures (stored_value_by_key st k = stored_value st s))
+  = lemma_get_slot_lookup_key st s k
+
+let lemma_as_map_stored_value (st:vstore{st.is_map}) (k:key)
+  : Lemma (requires (store_contains_key st k))
+          (ensures (stored_value_by_key st k = Spec.stored_value (as_map st) k))
+  = lemma_store_contains_key_inv st k;
+    Classical.exists_elim 
+      (stored_value_by_key st k = Spec.stored_value (as_map st) k) 
+      (Squash.get_proof (exists s. slot_key_equiv st s k)) 
+      (fun s -> lemma_slot_key_equiv_value st s k; 
+             lemma_as_map_slot_key_equiv st s k)
+   
