intermediate/Veritas.Intermediate.VerifySKC.fst
@@ -19,59 +19,60 @@ let vput (s:slot_id) (v:data_value) (vs: vtls {Valid? vs}) : vtls =
   else update_thread_store vs (update_store st s (DVal v))
 
 let vaddm (s:slot_id) (r:record) (s':slot_id) (vs: vtls {Valid? vs}): vtls =
-  let st = thread_store vs in
-  let (k,v) = r in
-  if not (s < Seq.length st.data) then Failed
-  (* check store contains slot s' *)
-  else if not (store_contains st s') then Failed
-  else
-    let k' = stored_key st s' in
-    let v' = stored_value st s' in
-    let a' = add_method_of st s' in
-    (* check k is a proper desc of k' *)
-    if not (is_proper_desc k k') then Failed
-    (* check store does not contain slot s *)
-    else if store_contains st s then Failed
-    (* check store does not contain key k
-       >> in lower levels we will check this via 'in_store' fields *)
-    else if store_contains_key st k then Failed
-    (* check type of v is consistent with k *)
-    else if not (is_value_of k v) then Failed
-    (* check v' is a merkle value *)
-    else if DVal? v' then Failed 
+  if not (s < thread_store_size vs) then Failed
+  else 
+    let st = thread_store vs in
+    let (k,v) = r in
+    (* check store contains slot s' *)
+    if not (store_contains st s') then Failed
     else
-      let v' = to_merkle_value v' in
-      let d = desc_dir k k' in
-      let dh' = desc_hash_dir v' d in 
-      let h = hashfn v in
-      match dh' with
-      | Empty -> (* k' has no child in direction d *)
-          (* first add must be init value *)
-          if v <> init_value k then Failed
-          else
-            let v'_upd = Spec.update_merkle_value v' d k h false in
-            let st_upd = update_store st s' (MVal v'_upd) in
-            let st_upd2 = add_to_store st_upd s k v Spec.MAdd in
-            update_thread_store vs st_upd2
-      | Desc k2 h2 b2 -> 
-          if k2 = k 
-          then (* k is a child of k' *)
-            (* check hashes match and k was not evicted to blum *)
-            if not (h2 = h && b2 = false) then Failed
-            else update_thread_store vs (add_to_store st s k v Spec.MAdd)
-          else (* otherwise, k is not a child of k' *)
-          (* first add must be init value *)
-          if v <> init_value k then Failed
-          (* check k2 is a proper desc of k *)
-          else if not (is_proper_desc k2 k) then Failed
-          else
-            let d2 = desc_dir k2 k in
-            let mv = to_merkle_value v in
-            let mv_upd = Spec.update_merkle_value mv d2 k2 h2 b2 in
-            let v'_upd = Spec.update_merkle_value v' d k h false in
-            let st_upd = update_store st s' (MVal v'_upd) in
-            let st_upd2 = add_to_store st_upd s k (MVal mv_upd) Spec.MAdd in
-            update_thread_store vs st_upd2
+      let k' = stored_key st s' in
+      let v' = stored_value st s' in
+      let a' = add_method_of st s' in
+      (* check k is a proper desc of k' *)
+      if not (is_proper_desc k k') then Failed
+      (* check store does not contain slot s *)
+      else if store_contains st s then Failed
+      (* check store does not contain key k
+         >> in lower levels we will check this via 'in_store' fields *)
+      else if store_contains_key st k then Failed
+      (* check type of v is consistent with k *)
+      else if not (is_value_of k v) then Failed
+      (* check v' is a merkle value *)
+      else if DVal? v' then Failed 
+      else
+        let v' = to_merkle_value v' in
+        let d = desc_dir k k' in
+        let dh' = desc_hash_dir v' d in 
+        let h = hashfn v in
+        match dh' with
+        | Empty -> (* k' has no child in direction d *)
+            (* first add must be init value *)
+            if v <> init_value k then Failed
+            else
+              let v'_upd = Spec.update_merkle_value v' d k h false in
+              let st_upd = update_store st s' (MVal v'_upd) in
+              let st_upd2 = add_to_store st_upd s k v Spec.MAdd in
+              update_thread_store vs st_upd2
+        | Desc k2 h2 b2 -> 
+            if k2 = k 
+            then (* k is a child of k' *)
+              (* check hashes match and k was not evicted to blum *)
+              if not (h2 = h && b2 = false) then Failed
+              else update_thread_store vs (add_to_store st s k v Spec.MAdd)
+            else (* otherwise, k is not a child of k' *)
+            (* first add must be init value *)
+            if v <> init_value k then Failed
+            (* check k2 is a proper desc of k *)
+            else if not (is_proper_desc k2 k) then Failed
+            else
+              let d2 = desc_dir k2 k in
+              let mv = to_merkle_value v in
+              let mv_upd = Spec.update_merkle_value mv d2 k2 h2 b2 in
+              let v'_upd = Spec.update_merkle_value v' d k h false in
+              let st_upd = update_store st s' (MVal v'_upd) in
+              let st_upd2 = add_to_store st_upd s k (MVal mv_upd) Spec.MAdd in
+              update_thread_store vs st_upd2
 
 (* key k is in store and was added using Merkle *)
 let is_instore_madd (st: vstore) (k: key): bool = 
@@ -118,12 +119,10 @@ let vevictm (s:slot_id) (s':slot_id) (vs: vtls {Valid? vs}): vtls =
             update_thread_store vs st_upd2
 
 let vaddb (s:slot_id) (r:record) (t:timestamp) (j:thread_id) (vs:vtls {Valid? vs}): vtls = 
-  (* epoch of timestamp of last evict *)
-  let e = MkTimestamp?.e t in
-  let st = thread_store vs in 
-  let (k,v) = r in
-  if not (s < Seq.length st.data) then Failed
-  else 
+  if not (s < thread_store_size vs) then Failed
+  else
+    let st = thread_store vs in 
+    let (k,v) = r in
     (* check value type consistent with key k *)
     if not (is_value_of k v) then Failed
     (* check store contains slot s *)
@@ -137,16 +136,12 @@ let vaddb (s:slot_id) (r:record) (t:timestamp) (j:thread_id) (vs:vtls {Valid? vs
       let clk = thread_clock vs in
       let clk_upd = Spec.max clk (next t) in
       let vs_upd2 = update_thread_clock vs_upd clk_upd in
-      (* check k is not in the store; update the valid flag accordingly *)
-      let valid = not (store_contains_key st k) in
-      let st_upd = {st with is_map=(st.is_map && valid)} in
       (* add record to store *)
-      let st_upd2 = add_to_store st_upd s k v Spec.BAdd in
-      update_thread_store vs_upd2 st_upd2
+      let st_upd = add_to_store st s k v Spec.BAdd in
+      update_thread_store vs_upd2 st_upd
 
 let vevictb (s:slot_id) (t:timestamp) (vs:vtls {Valid? vs}): vtls = 
   let clock = thread_clock vs in
-  let e = MkTimestamp?.e t in
   let st = thread_store vs in
   (* check store contains slot s *)
   if not (store_contains st s) then Failed
@@ -201,22 +196,19 @@ let vevictbm (s:slot_id) (s':slot_id) (t:timestamp) (vs:vtls {Valid? vs}): vtls 
             let st_upd = update_store st s' (MVal v'_upd) in
             vevictb s t (update_thread_store vs st_upd)
 
-let lemma_store_contains (st:vstore) (st':Spec.vstore) (s:slot_id) (k:key)
-  : Lemma (requires (store_rel st st' /\ slot_key_equiv st s k))
-          (ensures (store_contains st s = Spec.store_contains st' k))
-  = lemma_as_map_slot_key_equiv st s k
-
-let lemma_stored_value (st:vstore) (st':Spec.vstore) (s:slot_id) (k:data_key)
-  : Lemma (requires (store_rel st st' /\ slot_key_equiv st s k))
-          (ensures (Spec.store_contains st' k /\ stored_value st s = Spec.stored_value st' k))
-  = lemma_as_map_slot_key_equiv st s k
-
-let lemma_update_store (st:vstore) (st':Spec.vstore) (s:slot_id) (k:data_key) (v:data_value)
+let lemma_store_rel_update_store (st:vstore) (st':Spec.vstore) (s:slot_id) (k:data_key) (v:data_value)
   : Lemma (requires (store_rel st st' /\ slot_key_equiv st s k))
           (ensures (Spec.store_contains st' k /\
                     store_rel (update_store st s (DVal v)) (Spec.update_store st' k (DVal v))))
+          [SMTPat (store_rel st st'); SMTPat (update_store st s (DVal v)); SMTPat (Spec.update_store st' k (DVal v))]
   = lemma_as_map_slot_key_equiv st s k;
     admit()
+
+let lemma_add_to_store (st:vstore) (st':Spec.vstore) (s:st_index st) (k:key) (v:value_type_of k) (am:add_method)
+  : Lemma (requires (store_rel st st' /\ not (Spec.store_contains st' k)))
+          (ensures (store_rel (add_to_store st s k v am) (Spec.add_to_store st' k v am)))
+          [SMTPat (store_rel st st'); SMTPat (add_to_store st s k v am); SMTPat (Spec.add_to_store st' k v am)]
+  = admit()
 
 let lemma_vget_simulates_spec 
       (vs:vtls{Valid? vs})
@@ -226,15 +218,12 @@ let lemma_vget_simulates_spec
       (v:data_value)
   : Lemma (requires (vtls_rel vs vs' /\ slot_key_rel vs s k))
           (ensures (vtls_rel (vget s v vs) (Spec.vget k v vs')))
-  = let st = thread_store vs in
-    let st' = Spec.thread_store vs' in
-    lemma_store_contains st st' s k;
-    lemma_stored_value st st' s k
-
+  = ()
+  
 let lemma_vget_has_failed (vs:vtls{Valid? vs}) (s:slot_id) (v:data_value)
   : Lemma (requires (not (thread_store_is_map vs)))
           (ensures (has_failed (vget s v vs)))
-  = admit()
+  = ()
 
 let lemma_vput_simulates_spec 
       (vs:vtls{Valid? vs}) 
@@ -244,15 +233,12 @@ let lemma_vput_simulates_spec
       (v:data_value) 
   : Lemma (requires (vtls_rel vs vs' /\ slot_key_rel vs s k))
           (ensures (vtls_rel (vput s v vs) (Spec.vput k v vs'))) 
-  = let st = thread_store vs in
-    let st' = Spec.thread_store vs' in
-    lemma_store_contains st st' s k;
-    lemma_update_store st st' s k v
+  = ()
 
 let lemma_vput_has_failed (vs:vtls{Valid? vs}) (s:slot_id) (v:data_value)
   : Lemma (requires (not (thread_store_is_map vs)))
           (ensures (has_failed (vput s v vs)))
-  = admit()
+  = ()
 
 let lemma_vaddm_simulates_spec 
       (vs:vtls{Valid? vs}) 
@@ -260,7 +246,7 @@ let lemma_vaddm_simulates_spec
       (s s':slot_id)
       (r:record)
       (k':merkle_key)  
-  : Lemma (requires (vtls_rel vs vs') /\ slot_key_rel vs s' k')
+   : Lemma (requires (s < thread_store_size vs /\ vtls_rel vs vs' /\ slot_key_rel vs s' k'))
           (ensures (vtls_rel (vaddm s r s' vs) (Spec.vaddm r k' vs'))) 
   = let st = thread_store vs in
     let st' = Spec.thread_store vs' in
@@ -295,14 +281,16 @@ let lemma_vaddb_simulates_spec
       (r:record)
       (t:timestamp)
       (j:thread_id)
-  : Lemma (requires (vtls_rel vs vs'))
-          (ensures (vtls_rel (vaddb s r t j vs) (Spec.vaddb r t j vs'))) 
-  = admit()
+  : Lemma (requires (s < thread_store_size vs /\ 
+                     not (store_contains (thread_store vs) s) /\ 
+                     vtls_rel vs vs'))
+          (ensures (vtls_rel (vaddb s r t j vs) (Spec.vaddb r t j vs')))
+  = ()
 
 let lemma_vaddb_has_failed (vs:vtls{Valid? vs}) (s:slot_id) (r:record) (t:timestamp) (j:thread_id)
   : Lemma (requires (not (thread_store_is_map vs)))
           (ensures (has_failed (vaddb s r t j vs)))
-  = admit()
+  = ()
 
 let lemma_vevictb_simulates_spec 
       (vs:vtls{Valid? vs}) 
@@ -337,7 +325,7 @@ let lemma_vevictbm_has_failed (vs:vtls{Valid? vs}) (s s':slot_id) (t:timestamp)
 
 // TODO: what should the initial size be?
 let store_size = 65536 // 2 ^ 16
-let empty_store:vstore = { data=Seq.create store_size None; is_map=true }
+let empty_store:vstore = VStore (Seq.create store_size None) true
 
 (* Initialize verifier state *)
 let init_thread_state (id:thread_id): vtls = 
@@ -350,11 +338,22 @@ let init_thread_state (id:thread_id): vtls =
 
 let init_thread_state_valid (id:thread_id)
   : Lemma (Valid? (init_thread_state id))
-  = admit()
+  = ()
+
+let lemma_empty_store_rel () 
+  : Lemma (store_rel empty_store Spec.empty_store)
+  = lemma_as_map_empty store_size
 
 let lemma_init_thread_state_rel (id:thread_id)
   : Lemma (vtls_rel (init_thread_state id) (Spec.init_thread_state id))
-  = admit()
+  = let vs = Valid id empty_store (MkTimestamp 0 0) empty_hash_value empty_hash_value in 
+    let vs' = Spec.Valid id Spec.empty_store (MkTimestamp 0 0) Root empty_hash_value empty_hash_value in
+    lemma_empty_store_rel ();
+    if id = 0 
+    then 
+      let st = thread_store vs in
+      let st' = Spec.thread_store vs' in
+      lemma_add_to_store st st' 0 Root (init_value Root) Spec.MAdd
 
 let lemma_t_verify_step_simulates_spec (vs:vtls) (vs':Spec.vtls) (e:logSK_entry) (e':logK_entry)
   : Lemma (requires (vtls_rel vs vs' /\ (has_failed vs \/ log_entry_rel vs e e')))
@@ -387,6 +386,24 @@ let lemma_t_verify_step_simulates_spec (vs:vtls) (vs':Spec.vtls) (e:logSK_entry)
       | EvictB_SK s _ t -> lemma_vevictb_has_failed vs s t
       | EvictBM_SK s _ s' _ t -> lemma_vevictbm_has_failed vs s s' t
 
+let rec lemma_t_verify_aux_Failed (l:logSK)
+  : Lemma (ensures (t_verify_aux Failed l == Failed))
+          (decreases (Seq.length l))
+  = let n = Seq.length l in
+    if n <> 0
+    then 
+      let l' = prefix l (n - 1) in
+      lemma_t_verify_aux_Failed l'
+
+let rec lemma_t_verify_aux_Spec_Failed (l:logK)
+  : Lemma (ensures (Spec.t_verify_aux Spec.Failed l == Spec.Failed))
+          (decreases (Seq.length l))
+  = let n = Seq.length l in
+    if n <> 0
+    then 
+      let l' = prefix l (n - 1) in
+      lemma_t_verify_aux_Spec_Failed l'
+
 let rec lemma_t_verify_aux_simulates_spec (vs:vtls) (vs':Spec.vtls) (l:logSK) (l':logK)
   : Lemma (requires (vtls_rel vs vs' /\ Seq.length l = Seq.length l' /\ (Valid? vs ==> log_rel_with_vtls vs l l')))
           (ensures (vtls_rel (t_verify_aux vs l) (Spec.t_verify_aux vs' l')))
@@ -407,7 +424,10 @@ let rec lemma_t_verify_aux_simulates_spec (vs:vtls) (vs':Spec.vtls) (l:logSK) (l
         lemma_t_verify_aux_simulates_spec vs vs' l2 l2';
         lemma_t_verify_step_simulates_spec vs2 vs2' e e' 
       )
-      else admit() // in this case, both results are Failed
+      else (
+        lemma_t_verify_aux_Failed l2;
+        lemma_t_verify_aux_Spec_Failed l2'
+      )
 
 let lemma_t_verify_simulates_spec (id:thread_id) (l:logSK) (l':logK)
   : Lemma (requires (log_rel l l'))
